<?xml version="1.0" encoding="utf-8"?>
<rdf:RDF
  xmlns:schema="http://schema.org/"
  xmlns:dct="http://purl.org/dc/terms/"
  xmlns:rdf="http://www.w3.org/1999/02/22-rdf-syntax-ns#"
  xmlns:rdfs="http://www.w3.org/2000/01/rdf-schema#"
>
  <rdf:Property rdf:about="http://schema.org/trailerWeight">
    <dct:source rdf:resource="http://www.w3.org/wiki/WebSchemas/SchemaDotOrgSources#Automotive_Ontology_Working_Group"/>
    <rdfs:label>trailerWeight</rdfs:label>
    <schema:domainIncludes rdf:resource="http://schema.org/Vehicle"/>
    <rdfs:comment><![CDATA[The permitted weight of a trailer attached to the vehicle.<br/><br/>

Typical unit code(s): KGM for kilogram, LBR for pound
* Note 1: You can indicate additional information in the <a class="localLink" href="http://schema.org/name">name</a> of the <a class="localLink" href="http://schema.org/QuantitativeValue">QuantitativeValue</a> node.
* Note 2: You may also link to a <a class="localLink" href="http://schema.org/QualitativeValue">QualitativeValue</a> node that provides additional information using <a class="localLink" href="http://schema.org/valueReference">valueReference</a>.
* Note 3: Note that you can use <a class="localLink" href="http://schema.org/minValue">minValue</a> and <a class="localLink" href="http://schema.org/maxValue">maxValue</a> to indicate ranges.]]></rdfs:comment>
    <schema:rangeIncludes rdf:resource="http://schema.org/QuantitativeValue"/>
    <schema:isPartOf rdf:resource="http://auto.schema.org"/>
  </rdf:Property>
  <rdf:Property rdf:about="http://schema.org/meetsEmissionStandard">
    <schema:rangeIncludes rdf:resource="http://schema.org/URL"/>
    <schema:rangeIncludes rdf:resource="http://schema.org/Text"/>
    <rdfs:comment>Indicates that the vehicle meets the respective emission standard.</rdfs:comment>
    <dct:source rdf:resource="http://www.w3.org/wiki/WebSchemas/SchemaDotOrgSources#Automotive_Ontology_Working_Group"/>
    <schema:domainIncludes rdf:resource="http://schema.org/Vehicle"/>
    <schema:rangeIncludes rdf:resource="http://schema.org/QualitativeValue"/>
    <schema:isPartOf rdf:resource="http://auto.schema.org"/>
    <rdfs:label>meetsEmissionStandard</rdfs:label>
  </rdf:Property>
  <rdf:Property rdf:about="http://schema.org/torque">
    <rdfs:comment><![CDATA[The torque (turning force) of the vehicle's engine.<br/><br/>

Typical unit code(s): NU for newton metre (N m), F17 for pound-force per foot, or F48 for pound-force per inch<br/><br/>

<ul>
<li>Note 1: You can link to information about how the given value has been determined (e.g. reference RPM) using the <a class="localLink" href="http://schema.org/valueReference">valueReference</a> property.</li>
<li>Note 2: You can use <a class="localLink" href="http://schema.org/minValue">minValue</a> and <a class="localLink" href="http://schema.org/maxValue">maxValue</a> to indicate ranges.</li>
</ul>
]]></rdfs:comment>
    <schema:rangeIncludes rdf:resource="http://schema.org/QuantitativeValue"/>
    <schema:domainIncludes rdf:resource="http://schema.org/EngineSpecification"/>
    <dct:source rdf:resource="http://www.w3.org/wiki/WebSchemas/SchemaDotOrgSources#Automotive_Ontology_Working_Group"/>
    <schema:isPartOf rdf:resource="http://auto.schema.org"/>
    <rdfs:label>torque</rdfs:label>
  </rdf:Property>
  <rdf:Property rdf:about="http://schema.org/emissionsCO2">
    <rdfs:comment>The CO2 emissions in g/km. When used in combination with a QuantitativeValue, put "g/km" into the unitText property of that value, since there is no UN/CEFACT Common Code for "g/km".</rdfs:comment>
    <schema:isPartOf rdf:resource="http://auto.schema.org"/>
    <schema:domainIncludes rdf:resource="http://schema.org/Vehicle"/>
    <schema:rangeIncludes rdf:resource="http://schema.org/Number"/>
    <dct:source rdf:resource="http://www.w3.org/wiki/WebSchemas/SchemaDotOrgSources#Automotive_Ontology_Working_Group"/>
    <rdfs:label>emissionsCO2</rdfs:label>
  </rdf:Property>
  <rdf:Property rdf:about="http://schema.org/weightTotal">
    <schema:rangeIncludes rdf:resource="http://schema.org/QuantitativeValue"/>
    <schema:domainIncludes rdf:resource="http://schema.org/Vehicle"/>
    <rdfs:label>weightTotal</rdfs:label>
    <schema:isPartOf rdf:resource="http://auto.schema.org"/>
    <rdfs:comment><![CDATA[The permitted total weight of the loaded vehicle, including passengers and cargo and the weight of the empty vehicle.<br/><br/>

Typical unit code(s): KGM for kilogram, LBR for pound<br/><br/>

<ul>
<li>Note 1: You can indicate additional information in the <a class="localLink" href="http://schema.org/name">name</a> of the <a class="localLink" href="http://schema.org/QuantitativeValue">QuantitativeValue</a> node.</li>
<li>Note 2: You may also link to a <a class="localLink" href="http://schema.org/QualitativeValue">QualitativeValue</a> node that provides additional information using <a class="localLink" href="http://schema.org/valueReference">valueReference</a>.</li>
<li>Note 3: Note that you can use <a class="localLink" href="http://schema.org/minValue">minValue</a> and <a class="localLink" href="http://schema.org/maxValue">maxValue</a> to indicate ranges.</li>
</ul>
]]></rdfs:comment>
    <dct:source rdf:resource="http://www.w3.org/wiki/WebSchemas/SchemaDotOrgSources#Automotive_Ontology_Working_Group"/>
  </rdf:Property>
  <rdf:Property rdf:about="http://schema.org/payload">
    <schema:rangeIncludes rdf:resource="http://schema.org/QuantitativeValue"/>
    <rdfs:label>payload</rdfs:label>
    <schema:domainIncludes rdf:resource="http://schema.org/Vehicle"/>
    <dct:source rdf:resource="http://www.w3.org/wiki/WebSchemas/SchemaDotOrgSources#Automotive_Ontology_Working_Group"/>
    <rdfs:comment><![CDATA[The permitted weight of passengers and cargo, EXCLUDING the weight of the empty vehicle.<br/><br/>

Typical unit code(s): KGM for kilogram, LBR for pound<br/><br/>

<ul>
<li>Note 1: Many databases specify the permitted TOTAL weight instead, which is the sum of <a class="localLink" href="http://schema.org/weight">weight</a> and <a class="localLink" href="http://schema.org/payload">payload</a></li>
<li>Note 2: You can indicate additional information in the <a class="localLink" href="http://schema.org/name">name</a> of the <a class="localLink" href="http://schema.org/QuantitativeValue">QuantitativeValue</a> node.</li>
<li>Note 3: You may also link to a <a class="localLink" href="http://schema.org/QualitativeValue">QualitativeValue</a> node that provides additional information using <a class="localLink" href="http://schema.org/valueReference">valueReference</a>.</li>
<li>Note 4: Note that you can use <a class="localLink" href="http://schema.org/minValue">minValue</a> and <a class="localLink" href="http://schema.org/maxValue">maxValue</a> to indicate ranges.</li>
</ul>
]]></rdfs:comment>
    <schema:isPartOf rdf:resource="http://auto.schema.org"/>
  </rdf:Property>
  <rdfs:Class rdf:about="http://schema.org/Motorcycle">
    <dct:source rdf:resource="http://www.w3.org/wiki/WebSchemas/SchemaDotOrgSources#Automotive_Ontology_Working_Group"/>
    <rdfs:label>Motorcycle</rdfs:label>
    <schema:isPartOf rdf:resource="http://auto.schema.org"/>
    <rdfs:comment>A motorcycle or motorbike is a single-track, two-wheeled motor vehicle.</rdfs:comment>
    <rdfs:subClassOf rdf:resource="http://schema.org/Vehicle"/>
  </rdfs:Class>
  <schema:CarUsageType rdf:about="http://schema.org/RentalVehicleUsage">
    <rdfs:label>RentalVehicleUsage</rdfs:label>
    <rdfs:comment>Indicates the usage of the vehicle as a rental car.</rdfs:comment>
    <schema:isPartOf rdf:resource="http://auto.schema.org"/>
    <dct:source rdf:resource="http://www.w3.org/wiki/WebSchemas/SchemaDotOrgSources#Automotive_Ontology_Working_Group"/>
  </schema:CarUsageType>
  <rdf:Property rdf:about="http://schema.org/engineType">
    <schema:rangeIncludes rdf:resource="http://schema.org/QualitativeValue"/>
    <rdfs:comment>The type of engine or engines powering the vehicle.</rdfs:comment>
    <schema:domainIncludes rdf:resource="http://schema.org/EngineSpecification"/>
    <schema:rangeIncludes rdf:resource="http://schema.org/URL"/>
    <schema:rangeIncludes rdf:resource="http://schema.org/Text"/>
    <schema:isPartOf rdf:resource="http://auto.schema.org"/>
    <rdfs:label>engineType</rdfs:label>
    <dct:source rdf:resource="http://www.w3.org/wiki/WebSchemas/SchemaDotOrgSources#Automotive_Ontology_Working_Group"/>
  </rdf:Property>
  <rdf:Property rdf:about="http://schema.org/bodyType">
    <schema:rangeIncludes rdf:resource="http://schema.org/QualitativeValue"/>
    <schema:isPartOf rdf:resource="http://auto.schema.org"/>
    <schema:domainIncludes rdf:resource="http://schema.org/Vehicle"/>
    <rdfs:comment>Indicates the design and body style of the vehicle (e.g. station wagon, hatchback, etc.).</rdfs:comment>
    <dct:source rdf:resource="http://www.w3.org/wiki/WebSchemas/SchemaDotOrgSources#Automotive_Ontology_Working_Group"/>
    <schema:rangeIncludes rdf:resource="http://schema.org/Text"/>
    <schema:rangeIncludes rdf:resource="http://schema.org/URL"/>
    <rdfs:label>bodyType</rdfs:label>
  </rdf:Property>
  <rdf:Property rdf:about="http://schema.org/wheelbase">
    <schema:rangeIncludes rdf:resource="http://schema.org/QuantitativeValue"/>
    <rdfs:comment><![CDATA[The distance between the centers of the front and rear wheels.<br/><br/>

Typical unit code(s): CMT for centimeters, MTR for meters, INH for inches, FOT for foot/feet]]></rdfs:comment>
    <rdfs:label>wheelbase</rdfs:label>
    <schema:domainIncludes rdf:resource="http://schema.org/Vehicle"/>
    <schema:isPartOf rdf:resource="http://auto.schema.org"/>
    <dct:source rdf:resource="http://www.w3.org/wiki/WebSchemas/SchemaDotOrgSources#Automotive_Ontology_Working_Group"/>
  </rdf:Property>
  <rdf:Property rdf:about="http://schema.org/vehicleSpecialUsage">
    <schema:isPartOf rdf:resource="http://auto.schema.org"/>
    <schema:rangeIncludes rdf:resource="http://schema.org/CarUsageType"/>
    <rdfs:label>vehicleSpecialUsage</rdfs:label>
    <dct:source rdf:resource="http://www.w3.org/wiki/WebSchemas/SchemaDotOrgSources#Automotive_Ontology_Working_Group"/>
    <schema:rangeIncludes rdf:resource="http://schema.org/Text"/>
    <schema:domainIncludes rdf:resource="http://schema.org/Vehicle"/>
    <rdfs:comment>Indicates whether the vehicle has been used for special purposes, like commercial rental, driving school, or as a taxi. The legislation in many countries requires this information to be revealed when offering a car for sale.</rdfs:comment>
  </rdf:Property>
  <rdf:Property rdf:about="http://schema.org/enginePower">
    <rdfs:label>enginePower</rdfs:label>
    <dct:source rdf:resource="http://www.w3.org/wiki/WebSchemas/SchemaDotOrgSources#Automotive_Ontology_Working_Group"/>
    <rdfs:comment><![CDATA[The power of the vehicle's engine.
    Typical unit code(s): KWT for kilowatt, BHP for brake horsepower, N12 for metric horsepower (PS, with 1 PS = 735,49875 W)<br/><br/>

<ul>
<li>Note 1: There are many different ways of measuring an engine's power. For an overview, see  <a href="http://en.wikipedia.org/wiki/Horsepower#Engine_power_test_codes">http://en.wikipedia.org/wiki/Horsepower#Engine<em>power</em>test_codes</a>.</li>
<li>Note 2: You can link to information about how the given value has been determined using the <a class="localLink" href="http://schema.org/valueReference">valueReference</a> property.</li>
<li>Note 3: You can use <a class="localLink" href="http://schema.org/minValue">minValue</a> and <a class="localLink" href="http://schema.org/maxValue">maxValue</a> to indicate ranges.</li>
</ul>
]]></rdfs:comment>
    <schema:isPartOf rdf:resource="http://auto.schema.org"/>
    <schema:rangeIncludes rdf:resource="http://schema.org/QuantitativeValue"/>
    <schema:domainIncludes rdf:resource="http://schema.org/EngineSpecification"/>
  </rdf:Property>
  <rdf:Property rdf:about="http://schema.org/modelDate">
    <dct:source rdf:resource="http://www.w3.org/wiki/WebSchemas/SchemaDotOrgSources#Automotive_Ontology_Working_Group"/>
    <rdfs:label>modelDate</rdfs:label>
    <schema:isPartOf rdf:resource="http://auto.schema.org"/>
    <schema:rangeIncludes rdf:resource="http://schema.org/Date"/>
    <schema:domainIncludes rdf:resource="http://schema.org/Vehicle"/>
    <rdfs:comment>The release date of a vehicle model (often used to differentiate versions of the same make and model).</rdfs:comment>
  </rdf:Property>
  <rdf:Property rdf:about="http://schema.org/fuelCapacity">
    <schema:isPartOf rdf:resource="http://auto.schema.org"/>
    <rdfs:label>fuelCapacity</rdfs:label>
    <rdfs:comment><![CDATA[The capacity of the fuel tank or in the case of electric cars, the battery. If there are multiple components for storage, this should indicate the total of all storage of the same type.<br/><br/>

Typical unit code(s): LTR for liters, GLL of US gallons, GLI for UK / imperial gallons, AMH for ampere-hours (for electrical vehicles).]]></rdfs:comment>
    <schema:rangeIncludes rdf:resource="http://schema.org/QuantitativeValue"/>
    <dct:source rdf:resource="http://www.w3.org/wiki/WebSchemas/SchemaDotOrgSources#Automotive_Ontology_Working_Group"/>
    <schema:domainIncludes rdf:resource="http://schema.org/Vehicle"/>
  </rdf:Property>
  <rdf:Property rdf:about="http://schema.org/acrissCode">
    <dct:source rdf:resource="http://www.w3.org/wiki/WebSchemas/SchemaDotOrgSources#Automotive_Ontology_Working_Group"/>
    <rdfs:label>acrissCode</rdfs:label>
    <rdfs:comment>The ACRISS Car Classification Code is a code used by many car rental companies, for classifying vehicles. ACRISS stands for Association of Car Rental Industry Systems and Standards.</rdfs:comment>
    <schema:domainIncludes rdf:resource="http://schema.org/Car"/>
    <schema:domainIncludes rdf:resource="http://schema.org/BusOrCoach"/>
    <schema:rangeIncludes rdf:resource="http://schema.org/Text"/>
    <schema:isPartOf rdf:resource="http://auto.schema.org"/>
  </rdf:Property>
  <rdf:Property rdf:about="http://schema.org/seatingCapacity">
    <rdfs:label>seatingCapacity</rdfs:label>
    <schema:domainIncludes rdf:resource="http://schema.org/Vehicle"/>
    <schema:isPartOf rdf:resource="http://auto.schema.org"/>
    <schema:rangeIncludes rdf:resource="http://schema.org/Number"/>
    <schema:rangeIncludes rdf:resource="http://schema.org/QuantitativeValue"/>
    <rdfs:comment><![CDATA[The number of persons that can be seated (e.g. in a vehicle), both in terms of the physical space available, and in terms of limitations set by law.<br/><br/>

Typical unit code(s): C62 for persons]]></rdfs:comment>
    <dct:source rdf:resource="http://www.w3.org/wiki/WebSchemas/SchemaDotOrgSources#Automotive_Ontology_Working_Group"/>
  </rdf:Property>
  <rdf:Property rdf:about="http://schema.org/roofLoad">
    <rdfs:comment><![CDATA[The permitted total weight of cargo and installations (e.g. a roof rack) on top of the vehicle.<br/><br/>

Typical unit code(s): KGM for kilogram, LBR for pound<br/><br/>

<ul>
<li>Note 1: You can indicate additional information in the <a class="localLink" href="http://schema.org/name">name</a> of the <a class="localLink" href="http://schema.org/QuantitativeValue">QuantitativeValue</a> node.</li>
<li>Note 2: You may also link to a <a class="localLink" href="http://schema.org/QualitativeValue">QualitativeValue</a> node that provides additional information using <a class="localLink" href="http://schema.org/valueReference">valueReference</a></li>
<li>Note 3: Note that you can use <a class="localLink" href="http://schema.org/minValue">minValue</a> and <a class="localLink" href="http://schema.org/maxValue">maxValue</a> to indicate ranges.</li>
</ul>
]]></rdfs:comment>
    <dct:source rdf:resource="http://www.w3.org/wiki/WebSchemas/SchemaDotOrgSources#Automotive_Ontology_Working_Group"/>
    <schema:rangeIncludes rdf:resource="http://schema.org/QuantitativeValue"/>
    <schema:domainIncludes rdf:resource="http://schema.org/BusOrCoach"/>
    <schema:domainIncludes rdf:resource="http://schema.org/Car"/>
    <rdfs:label>roofLoad</rdfs:label>
    <schema:isPartOf rdf:resource="http://auto.schema.org"/>
  </rdf:Property>
  <rdf:Property rdf:about="http://schema.org/tongueWeight">
    <schema:domainIncludes rdf:resource="http://schema.org/Vehicle"/>
    <dct:source rdf:resource="http://www.w3.org/wiki/WebSchemas/SchemaDotOrgSources#Automotive_Ontology_Working_Group"/>
    <schema:rangeIncludes rdf:resource="http://schema.org/QuantitativeValue"/>
    <schema:isPartOf rdf:resource="http://auto.schema.org"/>
    <rdfs:comment><![CDATA[The permitted vertical load (TWR) of a trailer attached to the vehicle. Also referred to as Tongue Load Rating (TLR) or Vertical Load Rating (VLR)<br/><br/>

Typical unit code(s): KGM for kilogram, LBR for pound<br/><br/>

<ul>
<li>Note 1: You can indicate additional information in the <a class="localLink" href="http://schema.org/name">name</a> of the <a class="localLink" href="http://schema.org/QuantitativeValue">QuantitativeValue</a> node.</li>
<li>Note 2: You may also link to a <a class="localLink" href="http://schema.org/QualitativeValue">QualitativeValue</a> node that provides additional information using <a class="localLink" href="http://schema.org/valueReference">valueReference</a>.</li>
<li>Note 3: Note that you can use <a class="localLink" href="http://schema.org/minValue">minValue</a> and <a class="localLink" href="http://schema.org/maxValue">maxValue</a> to indicate ranges.</li>
</ul>
]]></rdfs:comment>
    <rdfs:label>tongueWeight</rdfs:label>
  </rdf:Property>
  <rdf:Property rdf:about="http://schema.org/accelerationTime">
    <schema:rangeIncludes rdf:resource="http://schema.org/QuantitativeValue"/>
    <rdfs:comment><![CDATA[The time needed to accelerate the vehicle from a given start velocity to a given target velocity.<br/><br/>

Typical unit code(s): SEC for seconds<br/><br/>

<ul>
<li>Note: There are unfortunately no standard unit codes for seconds/0..100 km/h or seconds/0..60 mph. Simply use "SEC" for seconds and indicate the velocities in the <a class="localLink" href="http://schema.org/name">name</a> of the <a class="localLink" href="http://schema.org/QuantitativeValue">QuantitativeValue</a>, or use <a class="localLink" href="http://schema.org/valueReference">valueReference</a> with a <a class="localLink" href="http://schema.org/QuantitativeValue">QuantitativeValue</a> of 0..60 mph or 0..100 km/h to specify the reference speeds.</li>
</ul>
]]></rdfs:comment>
    <schema:isPartOf rdf:resource="http://auto.schema.org"/>
    <rdfs:label>accelerationTime</rdfs:label>
    <schema:domainIncludes rdf:resource="http://schema.org/Vehicle"/>
    <dct:source rdf:resource="http://www.w3.org/wiki/WebSchemas/SchemaDotOrgSources#Automotive_Ontology_Working_Group"/>
  </rdf:Property>
  <schema:CarUsageType rdf:about="http://schema.org/DrivingSchoolVehicleUsage">
    <dct:source rdf:resource="http://www.w3.org/wiki/WebSchemas/SchemaDotOrgSources#Automotive_Ontology_Working_Group"/>
    <schema:isPartOf rdf:resource="http://auto.schema.org"/>
    <rdfs:label>DrivingSchoolVehicleUsage</rdfs:label>
    <rdfs:comment>Indicates the usage of the vehicle for driving school.</rdfs:comment>
  </schema:CarUsageType>
  <rdf:Property rdf:about="http://schema.org/engineDisplacement">
    <rdfs:comment><![CDATA[The volume swept by all of the pistons inside the cylinders of an internal combustion engine in a single movement. <br/><br/>

Typical unit code(s): CMQ for cubic centimeter, LTR for liters, INQ for cubic inches
* Note 1: You can link to information about how the given value has been determined using the <a class="localLink" href="http://schema.org/valueReference">valueReference</a> property.
* Note 2: You can use <a class="localLink" href="http://schema.org/minValue">minValue</a> and <a class="localLink" href="http://schema.org/maxValue">maxValue</a> to indicate ranges.]]></rdfs:comment>
    <schema:isPartOf rdf:resource="http://auto.schema.org"/>
    <schema:rangeIncludes rdf:resource="http://schema.org/QuantitativeValue"/>
    <schema:domainIncludes rdf:resource="http://schema.org/EngineSpecification"/>
    <dct:source rdf:resource="http://www.w3.org/wiki/WebSchemas/SchemaDotOrgSources#Automotive_Ontology_Working_Group"/>
    <rdfs:label>engineDisplacement</rdfs:label>
  </rdf:Property>
  <schema:CarUsageType rdf:about="http://schema.org/TaxiVehicleUsage">
    <schema:isPartOf rdf:resource="http://auto.schema.org"/>
    <dct:source rdf:resource="http://www.w3.org/wiki/WebSchemas/SchemaDotOrgSources#Automotive_Ontology_Working_Group"/>
    <rdfs:label>TaxiVehicleUsage</rdfs:label>
    <rdfs:comment>Indicates the usage of the car as a taxi.</rdfs:comment>
  </schema:CarUsageType>
  <rdfs:Class rdf:about="http://schema.org/MotorizedBicycle">
    <rdfs:label>MotorizedBicycle</rdfs:label>
    <schema:isPartOf rdf:resource="http://auto.schema.org"/>
    <rdfs:comment>A motorized bicycle is a bicycle with an attached motor used to power the vehicle, or to assist with pedaling.</rdfs:comment>
    <rdfs:subClassOf rdf:resource="http://schema.org/Vehicle"/>
    <dct:source rdf:resource="http://www.w3.org/wiki/WebSchemas/SchemaDotOrgSources#Automotive_Ontology_Working_Group"/>
  </rdfs:Class>
  <rdf:Property rdf:about="http://schema.org/speed">
    <schema:rangeIncludes rdf:resource="http://schema.org/QuantitativeValue"/>
    <dct:source rdf:resource="http://www.w3.org/wiki/WebSchemas/SchemaDotOrgSources#Automotive_Ontology_Working_Group"/>
    <rdfs:comment><![CDATA[The speed range of the vehicle. If the vehicle is powered by an engine, the upper limit of the speed range (indicated by <a class="localLink" href="http://schema.org/maxValue">maxValue</a> should be the maximum speed achievable under regular conditions.<br/><br/>

Typical unit code(s): KMH for km/h, HM for mile per hour (0.447 04 m/s), KNT for knot<br/><br/>

*Note 1: Use <a class="localLink" href="http://schema.org/minValue">minValue</a> and <a class="localLink" href="http://schema.org/maxValue">maxValue</a> to indicate the range. Typically, the minimal value is zero.
* Note 2: There are many different ways of measuring the speed range. You can link to information about how the given value has been determined using the <a class="localLink" href="http://schema.org/valueReference">valueReference</a> property.]]></rdfs:comment>
    <schema:isPartOf rdf:resource="http://auto.schema.org"/>
    <rdfs:label>speed</rdfs:label>
    <schema:domainIncludes rdf:resource="http://schema.org/Vehicle"/>
  </rdf:Property>
  <rdfs:Class rdf:about="http://schema.org/BusOrCoach">
    <rdfs:subClassOf rdf:resource="http://schema.org/Vehicle"/>
    <rdfs:comment>A bus (also omnibus or autobus) is a road vehicle designed to carry passengers. Coaches are luxury busses, usually in service for long distance travel.</rdfs:comment>
    <dct:source rdf:resource="http://www.w3.org/wiki/WebSchemas/SchemaDotOrgSources#Automotive_Ontology_Working_Group"/>
    <rdfs:label>BusOrCoach</rdfs:label>
    <schema:isPartOf rdf:resource="http://auto.schema.org"/>
  </rdfs:Class>
  <rdfs:Class rdf:about="http://schema.org/CarUsageType">
    <rdfs:label>CarUsageType</rdfs:label>
    <schema:isPartOf rdf:resource="http://auto.schema.org"/>
    <rdfs:comment>A value indicating a special usage of a car, e.g. commercial rental, driving school, or as a taxi.</rdfs:comment>
    <dct:source rdf:resource="http://www.w3.org/wiki/WebSchemas/SchemaDotOrgSources#Automotive_Ontology_Working_Group"/>
    <rdfs:subClassOf rdf:resource="http://schema.org/QualitativeValue"/>
  </rdfs:Class>
</rdf:RDF>
