@prefix : <https://schema.org/> .
@prefix rdf: <http://www.w3.org/1999/02/22-rdf-syntax-ns#> .
@prefix rdfs: <http://www.w3.org/2000/01/rdf-schema#> .
@prefix xml: <http://www.w3.org/XML/1998/namespace> .
@prefix xsd: <http://www.w3.org/2001/XMLSchema#> .

:syllabusSections a rdf:Property ;
    rdfs:label "syllabusSections" ;
    :domainIncludes :Course ;
    :isPartOf <https://pending.schema.org> ;
    :rangeIncludes :Syllabus ;
    :source <https://github.com/schemaorg/schemaorg/issues/3281> ;
    rdfs:comment """Indicates (typically several) Syllabus entities that lay out what each section of the overall course will cover.""" .


:courseSchedule a rdf:Property ;
    rdfs:label "courseSchedule" ;
    :domainIncludes :CourseInstance ;
    :isPartOf <https://pending.schema.org> ;
    :rangeIncludes :Schedule ;
    :source <https://github.com/schemaorg/schemaorg/issues/3281> ;
    rdfs:comment """Represents the length and pace of a course, expressed as a [[Schedule]].""" .

# todo: skills



:totalHistoricalEnrollment a rdf:Property ;
    rdfs:label "totalHistoricalEnrollment" ;
    :domainIncludes :Course ;
    :isPartOf <https://pending.schema.org> ;
    :rangeIncludes :Integer ;
    :source <https://github.com/schemaorg/schemaorg/issues/3281> ;
    rdfs:comment """The total number of students that have enrolled in the history of the course.""" .


:financialAidEligible  :domainIncludes :Course .

# todo: availableLanguage, re Subtitles, closed captions, or other languages the course is offered in. 
# existing property extended:
:availableLanguage  :domainIncludes :Course .


:Syllabus a rdfs:Class ;
    rdfs:label "Syllabus" ;
    :isPartOf <https://pending.schema.org> ;
    :source <https://github.com/schemaorg/schemaorg/issues/3281> ;
    rdfs:comment "A syllabus that describes the material covered in a course, often with several such sections per [[Course]] so that a distinct [[timeRequired]] can be provided for that section of the [[Course]].";
    rdfs:subClassOf :LearningResource .
