@prefix : <https://schema.org/> .
@prefix rdf: <http://www.w3.org/1999/02/22-rdf-syntax-ns#> .
@prefix rdfs: <http://www.w3.org/2000/01/rdf-schema#> .
@prefix xml: <http://www.w3.org/XML/1998/namespace> .
@prefix xsd: <http://www.w3.org/2001/XMLSchema#> .

:PaymentMethodType
    a rdfs:Class ;
    :isPartOf <https://pending.schema.org> ;
    rdfs:label "PaymentMethodType" ;
    :source <https://github.com/schemaorg/schemaorg/issues/3537> ;
    rdfs:comment """The type of payment method, only for generic payment types, specific forms of payments, like card payment should be expressed using subclasses of PaymentMethod.""" ;
    rdfs:subClassOf :Enumeration .

:Cash a :PaymentMethodType ;
    rdfs:label "Cash" ;
    rdfs:comment "Payment using cash, on premises, equivalent to <code>http://purl.org/goodrelations/v1#Cash</code>." .

:ByBankTransferInAdvance a :PaymentMethodType ;
    rdfs:label "ByBankTransferInAdvance" ;
    rdfs:comment "Payment in advance by bank transfer, equivalent to <code>http://purl.org/goodrelations/v1#ByBankTransferInAdvance</code>." .

:ByInvoice a :PaymentMethodType ;
    rdfs:label "ByInvoice" ;
    rdfs:comment "Payment by invoice, typically after the goods were delivered, equivalent to <code>http://purl.org/goodrelations/v1#ByInvoice</code>." .

:CheckInAdvance  a :PaymentMethodType ;
    rdfs:label "CheckInAdvance" ;
    rdfs:comment "Payment in advance by sending a check, equivalent to <code>http://purl.org/goodrelations/v1#CheckInAdvance</code>." .

:COD a :PaymentMethodType ;
    rdfs:label "COD" ;
    rdfs:comment "Cash on Delivery (COD) payment, equivalent to <code>http://purl.org/goodrelations/v1#COD</code>." .

:DirectDebit a :PaymentMethodType ;
    rdfs:label "DirectDebit" ;
    rdfs:comment "Payment in advance by direct debit from the bank, equivalent to <code>http://purl.org/goodrelations/v1#DirectDebit</code>." .

:InStorePrepay a :PaymentMethodType ;
    rdfs:label "InStorePrepay" ;
    rdfs:comment "Payment in advance in some form of shop or kiosk for goods purchased online." .

:PhoneCarrierPayment a :PaymentMethodType ;
    rdfs:label "PhoneCarrierPayment" ;
    rdfs:comment "Payment by billing via the phone carrier." .

:paymentMethodType a rdf:Property ;
    rdfs:label "paymentMethodType" ;
    :domainIncludes :PaymentMethod ;
    :isPartOf <https://pending.schema.org> ;
    :rangeIncludes :PaymentMethodType ;
    :source <https://github.com/schemaorg/schemaorg/issues/3537> ;
    rdfs:comment "The type of a payment method." .



