@prefix : <https://schema.org/> .
@prefix rdf: <http://www.w3.org/1999/02/22-rdf-syntax-ns#> .
@prefix rdfs: <http://www.w3.org/2000/01/rdf-schema#> .
@prefix xml: <http://www.w3.org/XML/1998/namespace> .
@prefix xsd: <http://www.w3.org/2001/XMLSchema#> .

:Certification a rdfs:Class ;
	rdfs:label "Certification" ;
    :isPartOf <https://pending.schema.org> ;
    :source <https://github.com/schemaorg/schemaorg/issues/3230> ;	
    rdfs:comment """A Certification is an official and authoritative statement about a subject, for example a product, service, person, or organization. A certification is typically issued by an indendent certification body, for example a professional organization or government. It formally attests certain characteristics about the subject, for example Organizations can be ISO certified, Food products can be certified Organic or Vegan, a Person can be a certified professional, a Place can be certified for food processing. There are certifications for many domains: regulatory, organizational, recycling, food, efficiency, educational, ecological, etc. A certification is a form of credential, as are accreditations and licenses. Mapped from the [gs1:CertificationDetails](https://www.gs1.org/voc/CertificationDetails) class in the GS1 Web Vocabulary.""" ;
    rdfs:subClassOf :CreativeWork .

:auditDate a rdf:Property ;
    rdfs:label "auditDate" ;
    :domainIncludes :Certification ;
    :rangeIncludes :Date,
        :DateTime ;
    :source <https://github.com/schemaorg/schemaorg/issues/3230> ;
    rdfs:comment "Date when a certification was last audited. See also  [gs1:certificationAuditDate](https://www.gs1.org/voc/certificationAuditDate)." .
	
:certificationIdentification a rdf:Property ;
    rdfs:label "certificationIdentification" ;
    :domainIncludes :Certification ;
    :isPartOf <https://pending.schema.org> ;
    :rangeIncludes :DefinedTerm,
        :Text ;
    :source <https://github.com/schemaorg/schemaorg/issues/3230> ;
    rdfs:comment "Identifier of a certification instance (as registered with an independent certification body). Typically this identifier can be used to consult and verify the certification instance. See also [gs1:certificationIdentification](https://www.gs1.org/voc/certificationIdentification)." .

:certificationRating a rdf:Property ;
    rdfs:label "certificationRating" ;
    :domainIncludes :Certification ;
    :isPartOf <https://pending.schema.org> ;
    :rangeIncludes :Rating ;
    :source <https://github.com/schemaorg/schemaorg/issues/3230> ;
    rdfs:comment "Rating of a certification instance (as defined by an independent certification body). Typically this rating can be used to rate the level to which the requirements of the certification instance are fulfilled. See also [gs1:certificationValue](https://www.gs1.org/voc/certificationValue)." .

:CertificationStatusEnumeration a rdfs:Class ;
    rdfs:label "CertificationStatusEnumeration" ;
    :isPartOf <https://pending.schema.org> ;
    :source <https://github.com/schemaorg/schemaorg/issues/3230> ;
    rdfs:comment "Enumerates the different statuses of a Certification (Active and Inactive)." ;
    rdfs:subClassOf :Enumeration .	
	
:CertificationActive a :CertificationStatusEnumeration ;
    rdfs:label "CertificationActive" ;
    :isPartOf <https://pending.schema.org> ;
    :source <https://github.com/schemaorg/schemaorg/issues/3230> ;
    rdfs:comment "Specifies that a certification is active." .

:CertificationInactive a :CertificationStatusEnumeration ;
    rdfs:label "CertificationInactive" ;
    :isPartOf <https://pending.schema.org> ;
    :source <https://github.com/schemaorg/schemaorg/issues/3230> ;
    rdfs:comment "Specifies that a certification is inactive (no longer in effect)." .
	
:certificationStatus a rdf:Property ;
    rdfs:label "certificationStatus" ;
    :domainIncludes :Certification ;
    :rangeIncludes :CertificationStatusEnumeration;
    :source <https://github.com/schemaorg/schemaorg/issues/3230> ;
    rdfs:comment "Indicates the current status of a certification: active or inactive. See also  [gs1:certificationStatus](https://www.gs1.org/voc/certificationStatus)." .
	
:hasCertification a rdf:Property ;
	rdfs:label "hasCertification" ;
	:domainIncludes :Product,
		 :Organization,
		 :Person,
		 :Service,
		 :Place;
	:rangeIncludes :Certification;
	:source <https://github.com/schemaorg/schemaorg/issues/3230> ;
	rdfs:comment "Certification information about a product, organization, service, place, or person." .




