@prefix : <https://schema.org/> .
@prefix rdf: <http://www.w3.org/1999/02/22-rdf-syntax-ns#> .
@prefix rdfs: <http://www.w3.org/2000/01/rdf-schema#> .
@prefix xml: <http://www.w3.org/XML/1998/namespace> .
@prefix xsd: <http://www.w3.org/2001/XMLSchema#> .

# FinancialIncentive, the main class for all financial incentives.
:FinancialIncentive a rdfs:Class ;
    rdfs:label "FinancialIncentive" ;
    :isPartOf <https://pending.schema.org> ;
    :source <https://github.com/schemaorg/schemaorg/issues/3572> ;
    rdfs:comment """<p>Represents financial incentives for goods/services offered by an organization (or individual).</p>

<p>Typically contains the [[name]] of the incentive, the [[incentivizedItem]], the [[incentiveAmount]], the [[incentiveStatus]], [[incentiveType]], the [[provider]] of the incentive, and [[eligibleWithSupplier]].</p>

<p>Optionally contains criteria on whether the incentive is limited based on [[purchaseType]], [[purchasePriceLimit]], [[incomeLimit]], and the [[qualifiedExpense]].
    """ ;
    rdfs:subClassOf :Intangible .

:incentiveType a rdf:Property ;
    rdfs:label "incentiveType" ;
    :domainIncludes :FinancialIncentive ;
    :rangeIncludes :IncentiveType ;
    :isPartOf <https://pending.schema.org> ;
    :source <https://github.com/schemaorg/schemaorg/issues/3572> ;
    rdfs:comment "The type of incentive offered (tax credit/rebate, tax deduction, tax waiver, subsidies, etc.)." .

:incentiveStatus a rdf:Property ;
    rdfs:label "incentiveStatus" ;
    :domainIncludes :FinancialIncentive ;
    :rangeIncludes :IncentiveStatus ;
    :isPartOf <https://pending.schema.org> ;
    :source <https://github.com/schemaorg/schemaorg/issues/3572> ;
    rdfs:comment "The status of the incentive (active, on hold, retired, etc.)." .

:eligibleWithSupplier a rdf:Property ;
    rdfs:label "eligibleWithSupplier" ;
    :domainIncludes :FinancialIncentive ;
    :rangeIncludes :Organization ;
    :isPartOf <https://pending.schema.org> ;
    :source <https://github.com/schemaorg/schemaorg/issues/3572> ;
    rdfs:comment "The supplier of the incentivized item/service for which the incentive is valid for such as a utility company, merchant, or contractor." .

:incentiveAmount a rdf:Property ;
    rdfs:label "incentiveAmount" ;
    :domainIncludes :FinancialIncentive ;
    :rangeIncludes :UnitPriceSpecification,
        :LoanOrCredit,
        :QuantitativeValue ;
    :isPartOf <https://pending.schema.org> ;
    :source <https://github.com/schemaorg/schemaorg/issues/3572> ;
    rdfs:comment """Describes the amount that can be redeemed from this incentive.
    
<p>[[QuantitativeValue]]: Use this for incentives based on price (either raw amount or percentage-based). For a raw amount example, "You can claim $2,500 - $7,500 from the total cost of installation" would be represented as the following:</p>
    {
        "@type": "QuantitativeValue",
        “minValue”: 2500,
        “maxValue”: 7500,
        "unitCode": "USD"
    }
<p>[[QuantitivateValue]] can also be used for percentage amounts. In such cases, value is used to represent the incentive’s percentage, while maxValue represents a limit (if one exists) to that incentive. The unitCode should be 'P1' and the unitText should be '%', while valueReference should be used for holding the currency type. For example, "You can claim up to 30% of the total cost of installation, up to a maximum of $7,500" would be:</p>
    {
        "@type": "QuantitativeValue",
        "value": 30,
        "unitCode": "P1",
        "unitText": "%",
        “maxValue”: 7500,
        “valueReference”: “USD”
    }
<p>[[UnitPriceSpecification]]: Use this for incentives that are based on amounts rather than price. For example, a net metering rebate that pays $10/kWh, up to $1,000:</p>
    {
        "@type": "UnitPriceSpecification",
        "price": 10,
        "priceCurrency": "USD",
        "referenceQuantity": 1,
        "unitCode": "DO3",
        "unitText": "kw/h",
        "maxPrice": 1000,
        "description": "$10 / kwh up to $1000"
    }
<p>[[LoanOrCredit]]: Use for incentives that are loan based. For example, a loan of $4,000 - $50,000 with a repayment term of 10 years, interest free would look like:</p>
    {
        "@type": "LoanOrCredit",
        "loanTerm": {
                "@type":"QuantitativeValue",
                "value":"10",
                "unitCode": "ANN"
            },
        "amount":[
            {
                "@type": "QuantitativeValue",
                "Name":"fixed interest rate",
                "value":"0",
            },
        ],
        "amount":[
            {
                "@type": "MonetaryAmount",
                "Name":"min loan amount",
                "value":"4000",
                "currency":"CAD"
            },
            {
                "@type": "MonetaryAmount",
                "Name":"max loan amount",
                "value":"50000",
                "currency":"CAD"
            }
        ],
    }

In summary: <ul><li>Use [[QuantitativeValue]] for absolute/percentage-based incentives applied on the price of a good/service.</li>
<li>Use [[UnitPriceSpecification]] for incentives based on a per-unit basis (e.g. net metering).</li>
<li>Use [[LoanOrCredit]] for loans/credits.</li>
</ul>.""" .

:incentivizedItem a rdf:Property ;
    rdfs:label "incentivizedItem" ;
    :domainIncludes :FinancialIncentive ;
    :rangeIncludes :DefinedTerm,
        :Product ;
    :isPartOf <https://pending.schema.org> ;
    :source <https://github.com/schemaorg/schemaorg/issues/3572> ;
    rdfs:comment """The type or specific product(s) and/or service(s) being incentivized.
<p>DefinedTermSets are used for product and service categories such as the United Nations Standard Products and Services Code:</p>
    {
        "@type": "DefinedTerm",
        "inDefinedTermSet": "https://www.unspsc.org/",
        "termCode": "261315XX",
        "name": "Photovoltaic module"
    }

<p>For a specific product or service, use the Product type:</p>
    {
        "@type": "Product",
        "name": "Kenmore White 17\" Microwave",
    }
For multiple different incentivized items, use multiple [[DefinedTerm]] or [[Product]].""" .

:purchaseType a rdf:Property ;
    rdfs:label "purchaseType" ;
    :domainIncludes :FinancialIncentive ;
    :rangeIncludes :PurchaseType ;
    :isPartOf <https://pending.schema.org> ;
    :source <https://github.com/schemaorg/schemaorg/issues/3572> ;
    rdfs:comment "Optional. The type of purchase the consumer must make in order to qualify for this incentive." .

:purchasePriceLimit a rdf:Property ;
    rdfs:label "purchasePriceLimit" ;
    :domainIncludes :FinancialIncentive ;
    :rangeIncludes :MonetaryAmount ;
    :isPartOf <https://pending.schema.org> ;
    :source <https://github.com/schemaorg/schemaorg/issues/3572> ;
    rdfs:comment "Optional. The maximum price the item can have and still qualify for this offer." .

:incomeLimit a rdf:Property ;
    rdfs:label "incomeLimit" ;
    :domainIncludes :FinancialIncentive ;
    :rangeIncludes :MonetaryAmount,
        :Text ;
    :isPartOf <https://pending.schema.org> ;
    :source <https://github.com/schemaorg/schemaorg/issues/3572> ;
    rdfs:comment """Optional. Income limit for which the incentive is applicable for.
    
<p>If MonetaryAmount is specified, this should be based on annualized income (e.g. if an incentive is limited to those making <$114,000 annually):</p>
    {
        "@type": "MonetaryAmount",
        "maxValue": 114000,
        "currency": "USD",
    }

Use Text for incentives that are limited based on other criteria, for example if an incentive is only available to recipients making 120% of the median poverty income in their area.""" .

:qualifiedExpense a rdf:Property ;
    rdfs:label "qualifiedExpense" ;
    :domainIncludes :FinancialIncentive ;
    :rangeIncludes :IncentiveQualifiedExpenseType ;
    :isPartOf <https://pending.schema.org> ;
    :source <https://github.com/schemaorg/schemaorg/issues/3572> ;
    rdfs:comment "Optional. The types of expenses that are covered by the incentive. For example some incentives are only for the goods (tangible items) but the services (labor) are excluded." .

# Enumerations.

:IncentiveType a rdfs:Class ;
    rdfs:label "IncentiveType" ;
    :isPartOf <https://pending.schema.org> ;
    :source <https://github.com/schemaorg/schemaorg/issues/3572> ;
    rdfs:comment "Enumerates common financial incentives for products, including tax credits, tax deductions, rebates and subsidies, etc." ;
    rdfs:subClassOf :Enumeration .

:IncentiveTypeTaxCredit a :IncentiveType ;
    rdfs:label "IncentiveTypeTaxCredit" ;
    :isPartOf <https://pending.schema.org> ;
    :source <https://github.com/schemaorg/schemaorg/issues/3572> ;
    rdfs:comment "An incentive that directly reduces the amount of tax owed by the recipient." .

:IncentiveTypeTaxDeduction a :IncentiveType ;
    rdfs:label "IncentiveTypeTaxDeduction" ;
    :isPartOf <https://pending.schema.org> ;
    :source <https://github.com/schemaorg/schemaorg/issues/3572> ;
    rdfs:comment "An incentive that reduces the recipient's amount of taxable income." .

:IncentiveTypeRebateOrSubsidy a :IncentiveType ;
    rdfs:label "IncentiveTypeRebateOrSubsidy" ;
    :isPartOf <https://pending.schema.org> ;
    :source <https://github.com/schemaorg/schemaorg/issues/3572> ;
    rdfs:comment "An incentive that reduces the purchase/lease cost of the good/service in question." .

:IncentiveTypeTaxWaiver a :IncentiveType ;
    rdfs:label "IncentiveTypeTaxWaiver" ;
    :isPartOf <https://pending.schema.org> ;
    :source <https://github.com/schemaorg/schemaorg/issues/3572> ;
    rdfs:comment "An incentive that reduces/exempts the recipient from taxation applicable to the incentivized good/service (e.g. luxury taxes, registration taxes, circulation tax)." .

:IncentiveTypeLoan a :IncentiveType ;
    rdfs:label "IncentiveTypeLoan" ;
    :isPartOf <https://pending.schema.org> ;
    :source <https://github.com/schemaorg/schemaorg/issues/3572> ;
    rdfs:comment "An incentive where the recipient can receive additional funding for the purchase/lease of the good/service, which must be paid back." .

:IncentiveStatus a rdfs:Class ;
    rdfs:label "IncentiveStatus" ;
    :isPartOf <https://pending.schema.org> ;
    :source <https://github.com/schemaorg/schemaorg/issues/3572> ;
    rdfs:comment "Enumerates a status for an incentive, such as whether it is active." ;
    rdfs:subClassOf :Enumeration .

:IncentiveStatusActive a :IncentiveStatus ;
    rdfs:label "IncentiveStatusActive" ;
    :isPartOf <https://pending.schema.org> ;
    :source <https://github.com/schemaorg/schemaorg/issues/3572> ;
    rdfs:comment "This incentive is currently active." .

:IncentiveStatusOnHold a :IncentiveStatus ;
    rdfs:label "IncentiveStatusOnHold" ;
    :isPartOf <https://pending.schema.org> ;
    :source <https://github.com/schemaorg/schemaorg/issues/3572> ;
    rdfs:comment "This incentive is currently active, but may not be accepting new applicants (e.g. max number of redemptions reached for a year)" .

:IncentiveStatusInDevelopment a :IncentiveStatus ;
    rdfs:label "IncentiveStatusInDevelopment" ;
    :isPartOf <https://pending.schema.org> ;
    :source <https://github.com/schemaorg/schemaorg/issues/3572> ;
    rdfs:comment "This incentive is currently being developed, and may become active/retired in the future." .

:IncentiveStatusRetired a :IncentiveStatus ;
    rdfs:label "IncentiveStatusRetired" ;
    :isPartOf <https://pending.schema.org> ;
    :source <https://github.com/schemaorg/schemaorg/issues/3572> ;
    rdfs:comment "This incentive is not longer available." .

:PurchaseType a rdfs:Class ;
    rdfs:label "PurchaseType" ;
    :isPartOf <https://pending.schema.org> ;
    :source <https://github.com/schemaorg/schemaorg/issues/3572> ;
    rdfs:comment "Enumerates a purchase type for an item." ;
    rdfs:subClassOf :Enumeration .

:PurchaseTypeNewPurchase a :PurchaseType ;
    rdfs:label "PurchaseTypeNewPurchase" ;
    :isPartOf <https://pending.schema.org> ;
    :source <https://github.com/schemaorg/schemaorg/issues/3572> ;
    rdfs:comment "This is a purchase of a new item." .

:PurchaseTypeUsedPurchase a :PurchaseType ;
    rdfs:label "PurchaseTypeUsedPurchase" ;
    :isPartOf <https://pending.schema.org> ;
    :source <https://github.com/schemaorg/schemaorg/issues/3572> ;
    rdfs:comment "This is a purchase of a used item." .

:PurchaseTypeLease a :PurchaseType ;
    rdfs:label "PurchaseTypeLease" ;
    :isPartOf <https://pending.schema.org> ;
    :source <https://github.com/schemaorg/schemaorg/issues/3572> ;
    rdfs:comment "This is a lease of an item." .

:PurchaseTypeTradeIn a :PurchaseType ;
    rdfs:label "PurchaseTypeTradeIn" ;
    :isPartOf <https://pending.schema.org> ;
    :source <https://github.com/schemaorg/schemaorg/issues/3572> ;
    rdfs:comment "This is a trade-in for an item." .

:IncentiveQualifiedExpenseType a rdfs:Class ;
    rdfs:label "IncentiveQualifiedExpenseType" ;
    :isPartOf <https://pending.schema.org> ;
    :source <https://github.com/schemaorg/schemaorg/issues/3572> ;
    rdfs:comment "The types of expenses that are covered by the incentive. For example some incentives are only for the goods (tangible items) but the services (labor) are excluded." ;
    rdfs:subClassOf :Enumeration .

:IncentiveQualifiedExpenseTypeGoodsOnly a :IncentiveQualifiedExpenseType ;
    rdfs:label "IncentiveQualifiedExpenseTypeGoodsOnly" ;
    :isPartOf <https://pending.schema.org> ;
    :source <https://github.com/schemaorg/schemaorg/issues/3572> ;
    rdfs:comment "This incentive applies to goods only." .

:IncentiveQualifiedExpenseTypeServicesOnly a :IncentiveQualifiedExpenseType ;
    rdfs:label "IncentiveQualifiedExpenseTypeServicesOnly" ;
    :isPartOf <https://pending.schema.org> ;
    :source <https://github.com/schemaorg/schemaorg/issues/3572> ;
    rdfs:comment "This incentive applies to services only." .

:IncentiveQualifiedExpenseTypeGoodsOrServices a :IncentiveQualifiedExpenseType ;
    rdfs:label "IncentiveQualifiedExpenseTypeGoodsOrServices" ;
    :isPartOf <https://pending.schema.org> ;
    :source <https://github.com/schemaorg/schemaorg/issues/3572> ;
    rdfs:comment "This incentive can apply to either goods or services (or both)." .

:IncentiveQualifiedExpenseTypeUtilityBill a :IncentiveQualifiedExpenseType ;
    rdfs:label "IncentiveQualifiedExpenseTypeUtilityBill" ;
    :isPartOf <https://pending.schema.org> ;
    :source <https://github.com/schemaorg/schemaorg/issues/3572> ;
    rdfs:comment "This incentive applies to utility bills." .


# Additions to existing types.
:provider :domainIncludes :FinancialIncentive.
:publisher :domainIncludes :FinancialIncentive.

:areaServed :domainIncludes :FinancialIncentive.

:validFrom :domainIncludes :FinancialIncentive.
:validThrough :domainIncludes :FinancialIncentive.