@prefix : <https://schema.org/> .
@prefix rdf: <http://www.w3.org/1999/02/22-rdf-syntax-ns#> .
@prefix rdfs: <http://www.w3.org/2000/01/rdf-schema#> .
@prefix xml: <http://www.w3.org/XML/1998/namespace> .
@prefix xsd: <http://www.w3.org/2001/XMLSchema#> .


:PlayGameAction a rdfs:Class ;
    rdfs:label "PlayGameAction" ;
    :isPartOf <https://pending.schema.org> ;
    :source <https://github.com/schemaorg/schemaorg/issues/3058> ;
    rdfs:comment "The act of playing a video game." ;
    rdfs:subClassOf :ConsumeAction .

:gameAvailabilityType a rdf:Property ;
    rdfs:label "gameAvailabilityType" ;
    :domainIncludes :PlayGameAction ;
    :rangeIncludes :Text, :GameAvailabilityEnumeration ;
    :isPartOf <https://pending.schema.org> ;
    :source <https://github.com/schemaorg/schemaorg/issues/3058>;
    rdfs:comment "Indicates the availability type of the game content associated with this action, such as whether it is a full version or a demo." .


:GameAvailabilityEnumeration a rdfs:Class ;
    rdfs:label "GameAvailabilityEnumeration" ;
    :isPartOf <https://pending.schema.org> ;
    :source <https://github.com/schemaorg/schemaorg/issues/3058> ;
    rdfs:comment "For a [[VideoGame]], such as used with a [[PlayGameAction]], an enumeration of the kind of game availability offered. " ;
    rdfs:subClassOf :Enumeration .

:FullGameAvailability a :GameAvailabilityEnumeration ;
    rdfs:label "FullGameAvailability" ;
    :isPartOf <https://pending.schema.org> ;
    :source <https://github.com/schemaorg/schemaorg/issues/3058> ;
    rdfs:comment "Indicates full game availability." .


:DemoGameAvailability a :GameAvailabilityEnumeration ;
    rdfs:label "DemoGameAvailability" ;
    :isPartOf <https://pending.schema.org> ;
    :source <https://github.com/schemaorg/schemaorg/issues/3058> ;
    rdfs:comment "Indicates demo game availability, i.e. a somehow limited demonstration of the full game." .

