@prefix : <https://schema.org/> .
@prefix rdf: <http://www.w3.org/1999/02/22-rdf-syntax-ns#> .
@prefix rdfs: <http://www.w3.org/2000/01/rdf-schema#> .
@prefix xml: <http://www.w3.org/XML/1998/namespace> .
@prefix xsd: <http://www.w3.org/2001/XMLSchema#> .

:PriceTypeEnumeration a rdfs:Class ;
    rdfs:label "PriceTypeEnumeration" ;
    :isPartOf <https://pending.schema.org> ;
    :source <https://github.com/schemaorg/schemaorg/issues/2712> ;
    rdfs:comment "Enumerates different price types, for example list price, invoice price, and sale price." ;
    rdfs:subClassOf :Enumeration .

:InvoicePrice a :PriceTypeEnumeration ;
    rdfs:label "InvoicePrice" ;
    :isPartOf <https://pending.schema.org> ;
    :source <https://github.com/schemaorg/schemaorg/issues/2712> ;
    rdfs:comment "Represents the invoice price of an offered product." .

:ListPrice a :PriceTypeEnumeration ;
    rdfs:label "ListPrice" ;
    :isPartOf <https://pending.schema.org> ;
    :source <https://github.com/schemaorg/schemaorg/issues/2712> ;
    rdfs:comment "Represents the list price (the price a product is actually advertised for) of an offered product." .

:MSRP a :PriceTypeEnumeration ;
    rdfs:label "MSRP" ;
    :isPartOf <https://pending.schema.org> ;
    :source <https://github.com/schemaorg/schemaorg/issues/2712> ;
    rdfs:comment "Represents the manufacturer suggested retail price (\"MSRP\") of an offered product." .

:MinimumAdvertisedPrice a :PriceTypeEnumeration ;
    rdfs:label "MinimumAdvertisedPrice" ;
    :isPartOf <https://pending.schema.org> ;
    :source <https://github.com/schemaorg/schemaorg/issues/2712> ;
    rdfs:comment "Represents the minimum advertised price (\"MAP\") (as dictated by the manufacturer) of an offered product." .

:SRP a :PriceTypeEnumeration ;
    rdfs:label "SRP" ;
    :isPartOf <https://pending.schema.org> ;
    :source <https://github.com/schemaorg/schemaorg/issues/2712> ;
    rdfs:comment "Represents the suggested retail price (\"SRP\") of an offered product." .

:SalePrice a :PriceTypeEnumeration ;
    rdfs:label "SalePrice" ;
    :isPartOf <https://pending.schema.org> ;
    :source <https://github.com/schemaorg/schemaorg/issues/2712> ;
    rdfs:comment "Represents a sale price (usually active for a limited period) of an offered product." .

:priceType :domainIncludes :CompoundPriceSpecification ;
    :rangeIncludes :PriceTypeEnumeration .

