@prefix : <http://schema.org/> .
@prefix rdf: <http://www.w3.org/1999/02/22-rdf-syntax-ns#> .
@prefix rdfs: <http://www.w3.org/2000/01/rdf-schema#> .

:FundingAgency a rdfs:Class ;
    rdfs:label "FundingAgency" ;
    :category "issue-383" ;
    :isPartOf <http://pending.schema.org> ;
    :source <https://www.w3.org/wiki/WebSchemas/SchemaDotOrgSources#FundInfoCollab> ;
    rdfs:comment """A FundingAgency is an organization that implements one or more [[FundingScheme]]s and manages
    the granting process (via [[Grant]]s, typically [[MonetaryGrant]]s).
    A funding agency is not always required for grant funding, e.g. philanthropic giving, corporate sponsorship etc.
    
    Examples of funding agencies include ERC, REA, NIH, Bill and Melinda Gates Foundation...
    """ ;
    rdfs:subClassOf :Project .

:FundingScheme a rdfs:Class ;
    rdfs:label "FundingScheme" ;
    :category "issue-383" ;
    :isPartOf <http://pending.schema.org> ;
    :source <https://www.w3.org/wiki/WebSchemas/SchemaDotOrgSources#FundInfoCollab> ;
    rdfs:comment """A FundingScheme combines organizational, project and policy aspects of grant-based funding
    that sets guidelines, principles and mechanisms to support other kinds of projects and activities.
    Funding is typically organized via [[Grant]] funding. Examples of funding schemes: Swiss Priority Programmes (SPPs); EU Framework 7 (FP7); Horizon 2020; the NIH-R01 Grant Program; Wellcome institutional strategic support fund. For large scale public sector funding, the management and administration of grant awards is often handled by other, dedicated, organizations - [[FundingAgency]]s such as ERC, REA, ...""" ;
    rdfs:subClassOf :Organization .

:Grant a rdfs:Class ;
    rdfs:label "Grant" ;
    :category "issue-383" ;
    :isPartOf <http://pending.schema.org> ;
    :source <https://www.w3.org/wiki/WebSchemas/SchemaDotOrgSources#FundInfoCollab> ;
    rdfs:comment """A grant, typically financial or otherwise quantifiable, of resources. Typically a [[funder]] sponsors some [[MonetaryAmount]] to an [[Organization]] or [[Person]],
    sometimes not necessarily via a dedicated or long-lived [[Project]], resulting in one or more outputs, or [[fundedItem]]s. For financial sponsorship, indicate the [[funder]] of a [[MonetaryGrant]]. For non-financial support, indicate [[sponsor]] of [[Grant]]s of resources (e.g. office space).

Grants support  activities directed towards some agreed collective goals, often but not always organized as [[Project]]s. Long-lived projects are sometimes sponsored by a variety of grants over time, but it is also common for a project to be associated with a single grant.

The amount of a [[Grant]] is represented using [[amount]] as a [[MonetaryAmount]].
    """ ;
    rdfs:subClassOf :Intangible .

:MonetaryGrant a rdfs:Class ;
    rdfs:label "MonetaryGrant" ;
    :category "issue-383" ;
    :isPartOf <http://pending.schema.org> ;
    :source <https://www.w3.org/wiki/WebSchemas/SchemaDotOrgSources#FundInfoCollab> ;
    rdfs:comment "A monetary grant." ;
    rdfs:subClassOf :Grant .

:Project a rdfs:Class ;
    rdfs:label "Project" ;
    :category "issue-383" ;
    :isPartOf <http://pending.schema.org> ;
    :source <https://www.w3.org/wiki/WebSchemas/SchemaDotOrgSources#FundInfoCollab> ;
    rdfs:comment """An enterprise (potentially individual but typically collaborative), planned to achieve a particular aim.
Use properties from [[Organization]], [[subOrganization]]/[[parentOrganization]] to indicate project sub-structures. 
   """ ;
    rdfs:subClassOf :Organization .

:ResearchProject a rdfs:Class ;
    rdfs:label "ResearchProject" ;
    :category "issue-383" ;
    :isPartOf <http://pending.schema.org> ;
    :source <https://www.w3.org/wiki/WebSchemas/SchemaDotOrgSources#FundInfoCollab> ;
    rdfs:comment "A Research project." ;
    rdfs:subClassOf :Project .

:amount a rdf:Property ;
    :domainIncludes :MonetaryGrant .

:fundedItem a rdf:Property ;
    rdfs:label "fundedItem" ;
    :category "issue-1688",
        "issue-383" ;
    :inverseOf :funding ;    
    :domainIncludes :Grant ;
    :isPartOf <http://pending.schema.org> ;
    :rangeIncludes :CreativeWork, :Event, :MonetaryGrant, :Organization, :Person ;
    :source <https://github.com/schemaorg/schemaorg/issues/1950>,
        <https://github.com/schemaorg/schemaorg/issues/383>,
        <https://www.w3.org/wiki/WebSchemas/SchemaDotOrgSources#TP> ;
    rdfs:comment """Indicates an item funded or sponsored through a [[Grant]]. 
    
The range of items is not exclusive, as other types of things may have been funded, e.g. equipment described as [[IndividualProduct]]""" .

:funding a rdf:Property ;
    rdfs:label "funding" ;
    :category "issue-383" ;
    :inverseOf :fundedItem ;    
    :domainIncludes :CreativeWork, :Event, :MonetaryGrant, :Organization, :Person ;
    :isPartOf <http://pending.schema.org> ;
    :rangeIncludes :Grant ;
    :source <https://github.com/schemaorg/schemaorg/issues/383>,
        <https://www.w3.org/wiki/WebSchemas/SchemaDotOrgSources#TP> ;
    rdfs:comment """A [[Grant]] that directly or indirectly provide funding/sponsoring. 

This property can be combined with [[funder]] to directly indicate the [[FundingScheme]] or [[FundingAgency]] that provided the grant.
    
The list of types for using this property is not exclusive, as other types of things may have been funded, e.g. equipment described as a [[IndividualProduct]].""" .

:funder a rdf:Property ;
    :domainIncludes :MonetaryGrant .

:sponsor a rdf:Property ;
    :domainIncludes :Grant .

